\documentclass[fleqn]{article}
\usepackage[utf8]{inputenc}
\usepackage[margin=2cm]{geometry}

% maths
\usepackage{amsmath}
\usepackage{amssymb}
\usepackage{amsthm}

% bibliography
\usepackage[round, sort&compress]{natbib}
\usepackage{har2nat}
\bibliographystyle{agsm}

% custom header/footer
\usepackage{fancyhdr}
\pagestyle{fancy}
\renewcommand{\headrulewidth}{0pt}
\fancyhf{}
\rfoot{\textsf{\thepage}}
\lfoot{\textsf{Suzie Brown}}

% project-specific commands
\newcommand{\E}{\mathbb{E}}
\newcommand{\F}{\mathcal{F}_{t-1}}
\newcommand{\Mn}{\operatorname{Multinomial}}
\newcommand{\vt}[2][t]{v_{#1}^{(#2)}}
\newcommand{\wt}[2][t]{w_{#1}^{(#2)}}
\newcommand{\wbar}[2][t]{\bar{w}_{#1}^{(#2)}}

\newcommand{\myrule}{\\ \rule{\textwidth}{1pt}}

\title{Residual resampling in SMC}
\author{Suzie Brown}
\date{\today}

\begin{document}
\maketitle
\thispagestyle{fancy}

THIS DOCUMENT IS OBSOLETE. These calculations are reproduced (with corrections) in \texttt{resmn\_roundup\_210526}.\\
\hrule
\vspace{10pt}

The offspring counts are sampled according to:
\begin{align*}
& \vt{i} = \lfloor N \wt{i} \rfloor + X_i \\
& X_i \sim \Mn (N-k, (\wbar{1}, \dots, \wbar{N}))
\end{align*}
where $k := \sum_{i=1}^N \lfloor N \wt{i} \rfloor$ is the number of offspring assigned deterministically, and $\wbar{i} := \frac{N\wt{i} - \lfloor N \wt{i} \rfloor}{N - k}$ are the residual weights. Let us also define the residuals $r_i := N\wt{i} - \lfloor N \wt{i} \rfloor$. So $\sum_{i=1}^N r_i = N-k$.

The coalescence rate is defined as
\begin{equation*}
c_N(t) := \frac{1}{(N)_2} \sum_{i=1}^{N} (\vt{i})_2.
\end{equation*}
We will use $c_N^m(t)$ and $c_N^r(t)$ to denote the coalescence rates with multinomial and residual resampling respectively.
The expectation then comes out as
\begin{align*}
\E[(\vt{i})_2 |\F] &= \E[(\vt{i})^2 |\F] - \E[\vt{i} |\F] \\
&= \E[\lfloor N\wt{i} \rfloor^2 |\F] + 2 \E[\lfloor N\wt{i} \rfloor r_i |\F] + \E\left[ r_i \left(1 - \frac{r_i}{N-k} + r_i \right) |\F \right] - \E[N\wt{i} |\F] \\
&=\E[ \lfloor N\wt{i} \rfloor^2 |\F] - \E[ \lfloor N\wt{i} \rfloor |\F] + 2 \E[ \lfloor N\wt{i} \rfloor r_i |\F] + \E\left[ r_i^2 \left(1- \frac{1}{N-k} \right) |\F\right] \\
&= \E[ (N\wt{i})^2 |\F] - \E[ \lfloor N\wt{i} \rfloor |\F] - \E\left[ \frac{r_i^2}{N-k} |\F \right]
\end{align*}
so we get
\begin{align}
\E[c^r_N(t) |\F] &=  \frac{1}{(N)_2}  \sum_{i=1}^{N} \E[(\vt{i})_2 |\F ]\notag\\
&= \frac{N}{N-1} \sum_{i=1}^{N} \E[(\wt{i})^2 |\F] - \frac{1}{(N)_2} \sum_{i=1}^{N} \E\left[ \frac{r_i^2}{N-k} |\F \right] - \frac{1}{(N)_2} \E[k |\F] \notag\\
&= \E[c^{m}_N(t) |\F] \left( 1 + \frac{1}{N-1} \right) - \frac{1}{(N)_2}  \E\left[ \frac{\sum_{i=1}^{N} (N\wt{i} - \lfloor N\wt{i}\rfloor)^2}{\sum_{j=1}^{N} (N\wt{j} - \lfloor N\wt{j}\rfloor)} \middle|\F \right] \notag\\
&\qquad -\frac{1}{(N)_2} \E \left[ \sum_{i=1}^{N} \lfloor N\wt{i}\rfloor \middle|\F \right]
\label{eq:cNt_1}
\end{align}
\textbf{Sanity check:}\\
When the weights are all equal, $\wt{i} \equiv 1/N$, we should have $\E[c^r_N(t) |\F] = 0$ since each particle will have exactly one offspring so it is impossible for any lineages to coalesce. In this case we have $\E[c^{m}_N(t) |\F] = \sum_{i=1}^{N} \E[(\wt{i})^2 |\F] = 1/N$ for multinomial resampling. We also have that $N\wt{i} \equiv \lfloor N\wt{i} \rfloor \equiv 1$ and hence $r_i = 0$ and $k=N$. Thus the RHS comes out as
\begin{equation*}
\frac{1}{N}\frac{N}{N-1} - 0 - \frac{1}{(N)_2} N = \frac{1}{N-1} - \frac{1}{N-1} = 0
\end{equation*}
as expected.
\myrule \\%-------------------------------
We can write it in a different form by combining the second and third terms of \eqref{eq:cNt_1}:
\begin{align*}
&- \frac{1}{(N)_2}  \E\left[ \frac{\sum_{i=1}^{N} (N\wt{i} - \lfloor N\wt{i}\rfloor)^2}{\sum_{j=1}^{N} (N\wt{j} - \lfloor N\wt{j}\rfloor)} |\F \right] 
-\frac{1}{(N)_2} \E \left[ \sum_{k=1}^{N} \lfloor N\wt{k}\rfloor \middle|\F \right] \\
&=: - \frac{1}{(N)_2} \E[A |\F]
\end{align*}
Then
\begin{align*}
A &=
 \frac{\sum_{i=1}^{N} (N\wt{i} - \lfloor N\wt{i}\rfloor)^2}{\sum_{j=1}^{N} (N\wt{j} - \lfloor N\wt{j}\rfloor)} 
+ \sum_{k=1}^{N} \lfloor N\wt{k}\rfloor \\
&= \frac{\sum_{i=1}^{N} (N\wt{i} - \lfloor N\wt{i}\rfloor)^2 + \sum_{i=1}^N\sum_{k=1}^N \lfloor N\wt{k} \rfloor (N\wt{i}- \lfloor N\wt{i} \rfloor)}{\sum_{j=1}^{N} (N\wt{j} - \lfloor N\wt{j}\rfloor)} \\
&=: \frac{A^\prime}{\sum_{j=1}^{N} (N\wt{j} - \lfloor N\wt{j}\rfloor)} 
\end{align*}
Then
\begin{align*}
A^\prime &=
\sum_{i=1}^{N} (N\wt{i} - \lfloor N\wt{i}\rfloor)^2 + \sum_{i=1}^N\sum_{k=1}^N \lfloor N\wt{k} \rfloor (N\wt{i}- \lfloor N\wt{i} \rfloor)\\
&= \sum_{i=1}^{N} \left\{ \left(N\wt{i} - \lfloor N\wt{i}\rfloor \right)^2 + \lfloor N\wt{i} \rfloor \left(N\wt{i} - \lfloor N\wt{i}\rfloor \right)
+ \sum_{k\neq i} \lfloor N\wt{k} \rfloor \left(N\wt{i} - \lfloor N\wt{i}\rfloor \right) \right\}\\
&= \sum_{i=1}^{N} \left\{ (N\wt{i})^2 - N\wt{i} \lfloor N\wt{i} \rfloor 
+ \sum_{k\neq i} \lfloor N\wt{k} \rfloor \left(N\wt{i} - \lfloor N\wt{i}\rfloor \right) \right\}\\
 &= \sum_{i=1}^{N} \left\{ \left(N\wt{i} - \lfloor N\wt{i} \rfloor \right) \left( N\wt{i} + \sum_{k\neq i} \lfloor N\wt{k} \rfloor \right) \right\}
\end{align*}
So we have
%\begin{equation*}
%A = \frac{\sum_{i=1}^{N} \left\{ \left(N\wt{i} - \lfloor N\wt{i} \rfloor \right) \left( N\wt{i} + \sum_{k\neq i} \lfloor N\wt{i} \rfloor \right) \right\}}{\sum_{j=1}^{N} (N\wt{j} - \lfloor N\wt{j}\rfloor)} 
%\end{equation*}
\begin{align*}
\E[c^r_N(t) |\F] &=  \E[c^{m}_N(t) |\F] \left( 1 + \frac{1}{N-1} \right) \\
&\qquad- \frac{1}{(N)_2}  \E\left[ \frac{\sum_{i=1}^{N} \left(N\wt{i} - \lfloor N\wt{i} \rfloor \right) \left( N\wt{i} + \sum_{k\neq i} \lfloor N\wt{k} \rfloor \right) }{\sum_{j=1}^{N} \left(N\wt{j} - \lfloor N\wt{j}\rfloor\right)} \middle|\F \right]  
\end{align*}

\bibliography{smc.bib}
\end{document}