\documentclass{article}
\usepackage[utf8]{inputenc}
\usepackage[margin=2cm]{geometry}

\usepackage{graphicx}
\usepackage{enumitem}

% custom header/footer
\usepackage{fancyhdr}
\pagestyle{fancy}
\renewcommand{\headrulewidth}{0pt}
\fancyhf{}
\rfoot{\textsf{\thepage}}
\lfoot{\textsf{Suzie Brown}}

%annotations
\usepackage{color}
\usepackage{xspace}
\newcommand{\seb}[1]{\xspace\textcolor{red}{#1}\xspace}

% bibliography
\usepackage[round, sort&compress]{natbib}
\usepackage{har2nat}
\bibliographystyle{agsm}

% maths
\usepackage{amsmath}
\usepackage{amssymb}
\usepackage{amsthm}
\usepackage{bbm}
\newtheorem{theorem}{Theorem}
\newtheorem{lemma}{Lemma}
\newcommand{\Prob}{\mathbb{P}}
\newcommand{\E}{\mathbb{E}}
\newcommand{\Et}{\mathbb{E}_t}
\newcommand{\V}{\operatorname{Var}}
\newcommand{\I}[1]{\mathbbm{1}_{\{#1\}}}
\newcommand{\1}[1]{\mathbb{I}_{#1}}
\newcommand{\Mn}{\operatorname{Multinomial}}

\title{Weak convergence proof: an aside}
\author{Suzie Brown}

\begin{document}
\maketitle
\thispagestyle{fancy}

\begin{lemma}
For any $n \leq N \in \mathbb{N}$, for all $t>0$, define 
\begin{equation}
E_t := \left\{ c_N(t) < \frac{(N-3)_{n-3}}{N^{n-3}} \left( \alpha \left(1 + \frac{2}{N-2} \right) + B_n \right)^{-1} \right\} 
\end{equation}
where $\alpha$ and $B_n$ are positive constants as in equation whatever.
Then, for all $t>0$,
\begin{equation}
\lim_{N\to\infty} \Prob \left[  \bigcap_{r=1}^{\tau_N(t)} E_r \right] = 1 .
\end{equation}
\end{lemma}

\begin{proof}
\begin{equation}
\Prob \left[  \bigcap_{r=1}^{\tau_N(t)} E_r \right]
= 1 - \Prob \left[  \bigcup_{r=1}^{\tau_N(t)} E_r^c \right]
\geq 1 - \E \left[ \sum_{r=1}^{\tau_N(t)} \Prob [E_r^c] \right] .
\end{equation}
Using the generalised Markov inequality,
\begin{align}
\Prob [E_r^c] &= \Prob \left[ c_N(t) \geq \frac{(N-3)_{n-3}}{N^{n-3}} \left( \alpha \left(1 + \frac{2}{N-2} \right) + B_n \right)^{-1} \right] \notag\\
&\leq \E[c_N(r)^2] \frac{N^{2(n-3)}}{(N-3)_{n-3}^2} \left( \alpha \left(1 + \frac{2}{N-2} \right) + B_n \right)^2 .
\end{align}
Now
\begin{align}
\Prob \left[  \bigcap_{r=1}^{\tau_N(t)} E_r \right]
&\geq 1 - \E \left[  \sum_{r=1}^{\tau_N(t)} \E[c_N(r)^2] \frac{N^{2(n-3)}}{(N-3)_{n-3}^2} \left( \alpha \left(1 + \frac{2}{N-2} \right) + B_n \right)^2 \right] \notag\\
&= 1 - \frac{N^{2(n-3)}}{(N-3)_{n-3}^2} \left( \alpha \left(1 + \frac{2}{N-2} \right) + B_n \right)^2 
\E \left[ \sum_{r=1}^{\tau_N(t)} c_N(r)^2 \right] \notag\\
&\overset{N\to\infty}{\longrightarrow} 1 - (\alpha + B_n)^2 \times 0 = 1 .
\end{align}

\end{proof}




\end{document}