\documentclass{article}
\usepackage[utf8]{inputenc}
\usepackage[margin=2cm]{geometry}

\usepackage{graphicx}
\usepackage{enumitem}
\usepackage[nobreak]{mdframed} % The nobreak option should probably be set locally in the final document, since breaks may be required in longer theorems.

% custom header/footer
\usepackage{fancyhdr}
\pagestyle{fancy}
\renewcommand{\headrulewidth}{0pt}
\fancyhf{}
\rfoot{\textsf{\thepage}}
\lfoot{\textsf{Suzie Brown}}

%annotations
\usepackage{color}
\usepackage{xspace}
\newcommand{\seb}[1]{\xspace\textcolor{red}{#1}\xspace}

% bibliography
\usepackage[round, sort&compress]{natbib}
\usepackage{har2nat}
\bibliographystyle{agsm}

% maths
\usepackage{amsmath}
\usepackage{amssymb}
\usepackage{amsthm}
\usepackage[mathscr]{euscript}
\usepackage{bbm}
\newmdtheoremenv{theorem}{Theorem}
\newmdtheoremenv{lemma}{Lemma}
\newcommand{\Prob}{\mathbb{P}}
\newcommand{\E}{\mathbb{E}}
\newcommand{\Et}{\mathbb{E}_t}
\newcommand{\V}{\operatorname{Var}}
\newcommand{\I}[1]{\mathbbm{1}_{\{#1\}}}
\newcommand{\1}[1]{\mathbbm{1}_{#1}}
\newcommand{\Mn}{\operatorname{Multinomial}}

%\allowdisplaybreaks

\title{Weak convergence proof v.2 (neater) (in progress)}
\author{Suzie Brown}

\begin{document}
\maketitle
\thispagestyle{fancy}

\begin{lemma}\label{thm:cleanup1}
\begin{equation}
t^l - \left( \sum_{s=1}^{\tau_N(t)} c_N(s)^2 \right) \binom{l}{2} (t+1)^{l-2} 
\leq \sum_{s_1\neq\dots\neq s_l}^{\tau_N(t)} \prod_{j=1}^l c_N(s_j)
\leq t^l + c_N(\tau_N(t)) (t+1)^l .
\end{equation}
\end{lemma}

\begin{proof}
As pointed out in \citet[Equation (8)]{koskela2018}, 
\begin{equation}\label{eq:002}
\sum_{s_1\neq\dots\neq s_l}^{\tau_N(t)} \prod_{j=1}^l c_N(s_j)
\geq \left( \sum_{s=0}^{\tau_N(t)} c_N(s) \right)^l
        - \binom{l}{2} \left( \sum_{s=0}^{\tau_N(t)} c_N(s)^2 \right)
        \left( \sum_{s=0}^{\tau_N(t)} c_N(s) \right)^{l-2} .
\end{equation}
By definition of $\tau_N$, 
\begin{equation}\label{eq:003}
t 
\leq \sum_{s=0}^{\tau_N(t)} c_N(s) 
\leq t+1 .
\end{equation}
Substituting these bounds into the RHS of \eqref{eq:002} yields the lower bound.

It is a true fact that
\begin{equation}\label{eq:005}
\sum_{s_1\neq\dots\neq s_l}^{\tau_N(t)} \prod_{j=1}^l c_N(s_j)
\leq \left( \sum_{s=0}^{\tau_N(t)} c_N(s) \right)^l ,
\end{equation}
as can be seen by considering the multinomial expansion of the RHS.
This is further bounded by
\begin{equation}
\left( \sum_{s=0}^{\tau_N(t)} c_N(s) \right)^l
\leq \left( \sum_{s=0}^{\tau_N(t) -1} c_N(s) + c_N(\tau_N(t)) \right)^l
\leq \left[ t + c_N(\tau_N(t)) \right]^l ,
\end{equation}
again using the definition of $\tau_N$.
A binomial expansion yields
\begin{equation}
\left[ t + c_N(\tau_N(t)) \right]^l
= t^l + \sum_{i=0}^{l-1} \binom{l}{i} t^i c_N(\tau_N(t))^{l-i}
= t^l + c_N(\tau_N(t)) \sum_{i=0}^{l-1} \binom{l}{i} t^i c_N(\tau_N(t))^{l-1-i} ,
\end{equation}
then since $c_N(s) \leq 1$ for all $s$,
\begin{equation}
\sum_{i=0}^{l-1} \binom{l}{i} t^i c_N(\tau_N(t))^{l-1-i}
\leq \sum_{i=0}^{l-1} \binom{l}{i} t^i
\leq (t+1)^l .
\end{equation}
Putting this together yields the upper bound.
\end{proof}


\begin{lemma}\label{thm:cleanup2}
Let $B$ be a positive constant which may depend on $n$.
\begin{equation}
\sum_{s_1\neq\dots\neq s_l}^{\tau_N(t)} \prod_{j=1}^l 
        \left[ c_N(s_j) + B D_N(s_j) \right]
\leq \sum_{s_1\neq\dots\neq s_l}^{\tau_N(t)} \prod_{j=1}^l c_N(s_j)
        + \left( \sum_{s=1}^{\tau_N(t)} D_N(s) \right) (t+1)^{l-1} (1+B)^l .
\end{equation}
\end{lemma}

\begin{proof}
We start with a binomial expansion:
\begin{align}
\sum_{s_1\neq\dots\neq s_l}^{\tau_N(t)} \prod_{j=1}^l 
        \left[ c_N(s_j) + B D_N(s_j) \right]
&= \sum_{s_1\neq\dots\neq s_l}^{\tau_N(t)} \sum_{\mathcal{I} \subseteq [l]}
        B^{l-|\mathcal{I}|} \left( \prod_{i\in\mathcal{I}} c_N(s_i) \right)
        \left( \prod_{j\notin\mathcal{I}} D_N(s_j) \right) \notag\\
&= \sum_{\mathcal{I} \subseteq [l]} B^{l-|\mathcal{I}|}
        \sum_{s_1\neq\dots\neq s_l}^{\tau_N(t)}
        \left( \prod_{i\in\mathcal{I}} c_N(s_i) \right)
        \left( \prod_{j\notin\mathcal{I}} D_N(s_j) \right) \label{eq:010}
\end{align}
where $[l] := \{1,\dots,l\}$. Since the sum is over all permutations of $r_1,\dots,r_l$, we may arbitrarily choose an ordering for $\{1,\dots,l\}$ such that $\mathcal{I} = \{ 1,\dots, |\mathcal{I}| \}$:
\begin{equation}
\sum_{\mathcal{I} \subseteq [l]} B^{l-|\mathcal{I}|}
        \sum_{s_1\neq\dots\neq s_l}^{\tau_N(t)}
        \left( \prod_{i\in\mathcal{I}} c_N(s_i) \right)
        \left( \prod_{j\notin\mathcal{I}} D_N(s_j) \right)
= \sum_{I=0}^l \binom{l}{I} B^{l-I} \sum_{s_1\neq\dots\neq s_l}^{\tau_N(t)}
        \left( \prod_{i=1}^I c_N(s_i) \right)
        \left( \prod_{j=I+1}^l D_N(s_j) \right) .
\end{equation}
Separating the term $I=l$,
\begin{align}
\sum_{I=0}^l \binom{l}{I} B^{l-I} \sum_{s_1\neq\dots\neq s_l}^{\tau_N(t)}
        \left( \prod_{i=1}^I c_N(s_i) \right)
        &\left( \prod_{j=I+1}^l D_N(s_j) \right)
= \sum_{s_1\neq\dots\neq s_l}^{\tau_N(t)} \prod_{j=1}^l c_N(s_j) \notag\\
&\qquad+ \sum_{I=0}^{l-1} \binom{l}{I} B^{l-I} 
        \sum_{s_1\neq\dots\neq s_l}^{\tau_N(t)}
        \left( \prod_{i=1}^I c_N(s_i) \right) \left( \prod_{j=I+1}^l D_N(s_j) \right). \label{eq:012}
\end{align}
In the second line, there is always at least one $D_N$ term, and $c_N(s) \leq D_N(s)$ for all $s$, so we can write
\begin{align}
\sum_{I=0}^{l-1}\binom{l}{I} B^{l-I} \sum_{s_1\neq\dots\neq s_l}^{\tau_N(t)}
        \left( \prod_{i=1}^I c_N(s_i) \right) \left( \prod_{j=I+1}^l D_N(s_j) \right)
&\leq \sum_{I=0}^{l-1}\binom{l}{I} B^{l-I} 
        \sum_{s_1\neq\dots\neq s_l}^{\tau_N(t)}
        \left( \prod_{i=1}^{l-1} c_N(s_i) \right) D_N(s_l) \notag\\
&\leq \sum_{I=0}^{l-1}\binom{l}{I} B^{l-I} 
        \left( \sum_{s_1\neq\dots\neq s_{l-1}}^{\tau_N(t)} 
        \prod_{i=1}^{l-1} c_N(s_i) \right) 
        \sum_{s_l=1}^{\tau_N(t)} D_N(s_l) \notag\\
&\leq \sum_{I=0}^{l-1}\binom{l}{I} B^{l-I} (t+1)^{l-1}
        \sum_{s=1}^{\tau_N(t)} D_N(s) \label{eq:013}
\end{align}
using \eqref{eq:005} and \eqref{eq:003}.
Finally, by the Binomial Theorem,
\begin{equation}\label{eq:014}
\sum_{I=0}^{l-1}\binom{l}{I} B^{l-I} (t+1)^{l-1}
        \sum_{s=1}^{\tau_N(t)} D_N(s)
\leq \left( \sum_{s=1}^{\tau_N(t)} D_N(s) \right) (t+1)^{l-1} (1+B)^l ,
\end{equation}
which, together with \eqref{eq:012}, concludes the proof.
\end{proof}


\begin{lemma}\label{thm:cleanup3}
Let $B$ be a positive constant which may depend on $n$.
\begin{equation}
\sum_{s_1\neq\dots\neq s_l}^{\tau_N(t)} \prod_{j=1}^l 
        \left[ c_N(s_j) - B D_N(s_j) \right]
\geq \sum_{s_1\neq\dots\neq s_l}^{\tau_N(t)} \prod_{j=1}^l c_N(s_j)
        - \left( \sum_{s=1}^{\tau_N(t)} D_N(s) \right) (t+1)^{l-1} (1+B)^l .
\end{equation}
\end{lemma}

\begin{proof}
A binomial expansion and subsequent manipulation as in \eqref{eq:010}--\eqref{eq:012} gives
\begin{align}
\sum_{s_1\neq\dots\neq s_l}^{\tau_N(t)} \prod_{j=1}^l 
        \left[ c_N(s_j) - B D_N(s_j) \right]
&= \sum_{\mathcal{I} \subseteq [l]} (-B)^{l-|\mathcal{I}|}
        \sum_{s_1\neq\dots\neq s_l}^{\tau_N(t)}
        \left( \prod_{i\in\mathcal{I}} c_N(s_i) \right)
        \left( \prod_{j\notin\mathcal{I}} D_N(s_j) \right) \notag\\
&= \sum_{I=0}^l \binom{l}{I} (-B)^{l-I} 
        \sum_{s_1\neq\dots\neq s_l}^{\tau_N(t)}
        \left( \prod_{i=1}^I c_N(s_i) \right)
        \left( \prod_{j=I+1}^l D_N(s_j) \right) \notag\\
&= \sum_{s_1\neq\dots\neq s_l}^{\tau_N(t)} \prod_{j=1}^l c_N(s_j)
        + \sum_{I=0}^{l-1} \binom{l}{I} (-B)^{l-I} 
        \sum_{s_1\neq\dots\neq s_l}^{\tau_N(t)}
        \left( \prod_{i=1}^I c_N(s_i) \right) 
        \left( \prod_{j=I+1}^l D_N(s_j) \right) \notag\\
&\geq \sum_{s_1\neq\dots\neq s_l}^{\tau_N(t)} \prod_{j=1}^l c_N(s_j)
        - \sum_{I=0}^{l-1} \binom{l}{I} B^{l-I} 
        \sum_{s_1\neq\dots\neq s_l}^{\tau_N(t)}
        \left( \prod_{i=1}^I c_N(s_i) \right) \left( \prod_{j=I+1}^l D_N(s_j) \right)
\end{align}
where the last inequality just multiplies some positive terms by $-1$.
Then \eqref{eq:013}--\eqref{eq:014} can be applied directly (noting that an upper bound on negative terms gives a lower bound overall):
\begin{equation}
- \sum_{I=0}^{l-1} \binom{l}{I} B^{l-I} 
        \sum_{s_1\neq\dots\neq s_l}^{\tau_N(t)}
        \left( \prod_{i=1}^I c_N(s_i) \right) \left( \prod_{j=I+1}^l D_N(s_j) \right)
\geq \left( \sum_{s=1}^{\tau_N(t)} D_N(s) \right) (t+1)^{l-1} (1+B)^l 
\end{equation}
which concludes the proof.
\end{proof}


\begin{lemma}[Basis step]\label{thm:basis}
For any $0 < t < \infty$,
\begin{equation}
\lim_{N\to\infty} \E\left[ \prod_{r=1}^{\tau_N(t)} (1-p_r) \right] 
= e^{-\alpha_n t}
\end{equation}
where $\alpha_n := n(n-1)/2$.
\end{lemma}

\begin{proof}
We start by showing that
$\lim_{N\to\infty}\E\left[ \prod_{r=1}^{\tau_N(t)} (1-p_r) \right] 
\leq e^{-\alpha_n t}$.\\
From \citet[Lemma 1 Case 1]{koskela2018}, taking $\xi=\Delta$, we have
\begin{equation}
1-p_t 
= p_{\Delta\Delta}(t) \leq 1 - \alpha_n (1+O(N^{-1})) 
        \left[ c_N(t) - B_n^\prime D_N(t) \right] 
\end{equation}
where the $O(N^{-1})$ term does not depend on $t$.
Applying a multinomial expansion and then separating the positive and negative terms,
\begin{align}
\prod_{r=1}^{\tau_N(t)} (1-p_r)
&\leq 1 + \sum_{l=1}^{\tau_N(t)} (- \alpha_n)^l (1+O(N^{-1})) 
        \frac{1}{l!} \sum_{s_1\neq\dots\neq s_l}^{\tau_N(t)}\prod_{j=1}^l
        \left[ c_N(s_j) - B_n^\prime D_N(s_j) \right] \notag\\
&= 1 + \sum_{\substack{l=2 \\ \text{even} }}^{\tau_N(t)} 
        \alpha_n^l (1+O(N^{-1})) \frac{1}{l!} 
        \sum_{s_1\neq\dots\neq s_l}^{\tau_N(t)}\prod_{j=1}^l
        \left[ c_N(s_j) - B_n^\prime D_N(s_j) \right] \notag\\
    &\qquad- \sum_{\substack{l=1 \\ \text{odd} }}^{\tau_N(t)} 
        \alpha_n^l (1+O(N^{-1})) \frac{1}{l!} 
        \sum_{s_1\neq\dots\neq s_l}^{\tau_N(t)}\prod_{j=1}^l
        \left[ c_N(s_j) - B_n^\prime D_N(s_j) \right] .
\end{align}
This is further bounded by applying Lemma~\ref{thm:cleanup3} and then both bounds of Lemma~\ref{thm:cleanup1}:
\begin{align}
\prod_{r=1}^{\tau_N(t)} (1-p_r)
&\leq 1 + \sum_{\substack{l=2 \\ \text{even} }}^{\tau_N(t)} 
        \alpha_n^l (1+O(N^{-1})) \frac{1}{l!} 
        \sum_{s_1\neq\dots\neq s_l}^{\tau_N(t)}\prod_{j=1}^l c_N(s_j) \notag\\
    &\qquad- \sum_{\substack{l=1 \\ \text{odd} }}^{\tau_N(t)} 
        \alpha_n^l (1+O(N^{-1})) \frac{1}{l!} 
        \left\{ \sum_{s_1\neq\dots\neq s_l}^{\tau_N(t)}\prod_{j=1}^l c_N(s_j)
        - \left( \sum_{s=1}^{\tau_N(t)} D_N(s) \right) 
        (t+1)^{l-1} (1+B_n^\prime)^l \right\} \notag\\
&\leq 1 + \sum_{\substack{l=2 \\ \text{even} }}^{\tau_N(t)} 
        \alpha_n^l (1+O(N^{-1})) \frac{1}{l!} 
        \left\{ t^l + c_N(\tau_N(t)) (t+1)^l \right\} \notag\\
    &\qquad- \sum_{\substack{l=1 \\ \text{odd} }}^{\tau_N(t)} 
        \alpha_n^l (1+O(N^{-1})) \frac{1}{l!} 
        \left\{ t^l - \left( \sum_{s=1}^{\tau_N(t)} c_N(s)^2 \right) 
        \binom{l}{2} (t+1)^{l-2}
        - \left( \sum_{s=1}^{\tau_N(t)} D_N(s) \right) 
        (t+1)^{l-1} (1+B_n^\prime)^l \right\} .
\end{align}
A bit of tidying up and we have
\begin{align}
\prod_{r=1}^{\tau_N(t)} (1-p_r)
&\leq \sum_{l=0}^{\tau_N(t)} (-\alpha_n)^l (1+O(N^{-1})) \frac{1}{l!} t^l
    + c_N(\tau_N(t)) \sum_{\substack{l=2 \\ \text{even} }}^{\tau_N(t)}
        \alpha_n^l (1+O(N^{-1})) \frac{1}{l!} (t+1)^l \notag\\
    &\qquad+ \left( \sum_{s=1}^{\tau_N(t)} c_N(s)^2 \right)
        \sum_{\substack{l=1 \\ \text{odd} }}^{\tau_N(t)} \alpha_n^l
        (1+O(N^{-1})) \frac{1}{l!} \binom{l}{2} (t+1)^{l-2} \notag\\
    &\qquad+ \left( \sum_{s=1}^{\tau_N(t)} D_N(s) \right) 
        \sum_{\substack{l=1 \\ \text{odd} }}^{\tau_N(t)} \alpha_n^l
        (1+O(N^{-1})) \frac{1}{l!} (t+1)^{l-1} (1+B_n^\prime)^l \notag\\
&\leq \sum_{l=0}^{\tau_N(t)} (-\alpha_n)^l (1+O(N^{-1})) \frac{1}{l!} t^l
    + c_N(\tau_N(t)) \exp[ \alpha_n (1+O(N^{-1})) (t+1) ] \notag\\
    &\qquad+ \left( \sum_{s=1}^{\tau_N(t)} c_N(s)^2 \right)
        \frac{1}{2} \alpha_n^2 \exp[ \alpha_n (1+O(N^{-1})) (t+1) ] \notag\\
    &\qquad+ \left( \sum_{s=1}^{\tau_N(t)} D_N(s) \right)
        \exp[ \alpha_n (1+O(N^{-1})) (t+1) (1+B_n^\prime) ].
\end{align}
Now, taking the expectation and limit, and applying \citet[Equations (3.3)--(3.5)]{brown2021} and Lemma~?? \seb{(Lemma 2 in the messy weakconv note; not written up here yet)},
\begin{align}
\lim_{N\to\infty} \E \left[ \prod_{r=1}^{\tau_N(t)} (1-p_r) \right]
&\leq \sum_{l=0}^{\infty} (-\alpha_n)^l \frac{1}{l!} t^l
        \lim_{N\to\infty} \Prob \left[ \tau_N(t) \geq l \right]
    + \lim_{N\to\infty} \E \left[ c_N(\tau_N(t)) \right]
        \exp[ \alpha_n (t+1) ] \notag\\
    &\qquad+ \lim_{N\to\infty} \E \left[ \sum_{s=1}^{\tau_N(t)} 
        c_N(s)^2 \right]
        \frac{1}{2} \alpha_n^2 \exp[ \alpha_n (t+1) ] \notag\\
    &\qquad+ \lim_{N\to\infty} \E \left[ \sum_{s=1}^{\tau_N(t)} D_N(s) \right]
        \exp[ \alpha_n (t+1) (1+B_n^\prime) ] \notag\\
&= \sum_{l=0}^{\infty} (-\alpha_n)^l \frac{1}{l!} t^l
= e^{-\alpha_n t}. \label{eq:022}
\end{align}

It remains to show that
$\lim_{N\to\infty}\E\left[ \prod_{r=1}^{\tau_N(t)} (1-p_r) \right] 
\geq e^{-\alpha_n t}$.\\
From \citet[Equation (3.14)]{brown2021}, taking $\xi=\Delta$, we have
\begin{equation}
1-p_t 
= p_{\Delta\Delta}(t) \geq 1 - \alpha_n (1+O(N^{-1})) 
        \left[c_N(t) + B_n D_N(t) \right]
\end{equation}
where $B_n >0$ and the $O(N^{-1})$ term does not depend on $t$.
In particular,
\begin{equation}
1-p_t
= p_{\Delta\Delta}(t) \geq 1 - \frac{N^{n-2}}{(N-2)_{n-2}} \alpha_n c_N(t) 
        - \frac{N^{n-3}}{(N-3)_{n-3}} B_n D_N(t) .
\end{equation}
Since $D_N(s) \leq c_N(s)$ for all $s$ \citep[p.9]{koskela2018}, a sufficient condition for this bound to be non-negative is
\begin{equation}
E_r 
:= \left\{ c_N(r) \leq \frac{(N-3)_{n-3}}{N^{n-3}} 
        \left( \alpha_n \left(1 + \frac{2}{N-2} \right) + B_n \right)^{-1} \right\} ,
\end{equation}
and we define $E := \bigcap_{r=1}^{\tau_N(t)} E_r$.
We now apply a multinomial expansion to the product, and split into positive and negative terms:
\begin{align}
\prod_{r=1}^{\tau_N(t)} (1-p_r)
&\geq \left\{ 1 + \sum_{l=1}^{\tau_N(t)} (-\alpha_n)^l (1+O(N^{-1})) 
        \frac{1}{l!} \sum_{s_1\neq\dots\neq s_l}^{\tau_N(t)}\prod_{j=1}^l
        \left[ c_N(s_j) + B_n D_N(s_j) \right] \right\} \1{E} \notag\\
&= \Bigg\{ 1 + \sum_{\substack{l=2 \\ \text{even} }}^{\tau_N(t)} 
        \alpha_n^l (1+O(N^{-1})) \frac{1}{l!} 
        \sum_{s_1\neq\dots\neq s_l}^{\tau_N(t)}\prod_{j=1}^l
        \left[ c_N(s_j) + B_n D_N(s_j) \right] \notag\\
    &\qquad- \sum_{\substack{l=1 \\ \text{odd} }}^{\tau_N(t)} 
        \alpha_n^l (1+O(N^{-1})) \frac{1}{l!}
        \sum_{s_1\neq\dots\neq s_l}^{\tau_N(t)}\prod_{j=1}^l
        \left[ c_N(s_j) + B_n D_N(s_j) \right] \Bigg\} \1{E}
\end{align}
This is further bounded by applying Lemma~\ref{thm:cleanup2} and both bounds in Lemma~\ref{thm:cleanup1}:
\begin{align}
\prod_{r=1}^{\tau_N(t)} (1-p_r)
&\geq \Bigg\{ 1 + \sum_{\substack{l=2 \\ \text{even} }}^{\tau_N(t)} 
        \alpha_n^l (1+O(N^{-1})) \frac{1}{l!} 
        \sum_{s_1\neq\dots\neq s_l}^{\tau_N(t)}\prod_{j=1}^l c_N(s_j) \notag\\
    &\qquad- \sum_{\substack{l=1 \\ \text{odd} }}^{\tau_N(t)} 
        \alpha_n^l (1+O(N^{-1})) \frac{1}{l!}
        \left[ \sum_{s_1\neq\dots\neq s_l}^{\tau_N(t)}\prod_{j=1}^l c_N(s_j)
        + \left( \sum_{s=1}^{\tau_N(t)} D_N(s) \right)
        (t+1)^{l-1} (1+B_n)^l \right] \Bigg\} \1{E} \notag\\
&\geq \Bigg\{ 1 + \sum_{\substack{l=2 \\ \text{even} }}^{\tau_N(t)} 
        \alpha_n^l (1+O(N^{-1})) \frac{1}{l!} 
        \left[ t^l - \left( \sum_{s=1}^{\tau_N(t)} c_N(s)^2 \right)
        \binom{l}{2}(t+1)^{l-2} \right] \notag\\
    &\qquad- \sum_{\substack{l=1 \\ \text{odd} }}^{\tau_N(t)} 
        \alpha_n^l (1+O(N^{-1})) \frac{1}{l!}
        \left[ t^l + c_N(\tau_N(t)) (t+1)^l
        + \left( \sum_{s=1}^{\tau_N(t)} D_N(s) \right)
        (t+1)^{l-1} (1+B_n)^l \right] \Bigg\} \1{E} .
\end{align}
Tidying things up,
\begin{align}
\prod_{r=1}^{\tau_N(t)} (1-p_r)
&\geq \sum_{l=0}^{\tau_N(t)} (-\alpha_n)^l (1+O(N^{-1})) 
        \frac{1}{l!} t^l \1{E}
        - \left( \sum_{s=1}^{\tau_N(t)} c_N(s)^2 \right)
        \sum_{\substack{l=2 \\ \text{even} }}^{\tau_N(t)} 
        \alpha_n^l (1+O(N^{-1})) \frac{1}{l!} \binom{l}{2}(t+1)^{l-2} \notag\\
    &\qquad- c_N(\tau_N(t)) \sum_{\substack{l=1 \\ \text{odd} }}^{\tau_N(t)} 
        \alpha_n^l (1+O(N^{-1})) \frac{1}{l!} (t+1)^l \notag\\
    &\qquad- \left( \sum_{s=1}^{\tau_N(t)} D_N(s) \right)
        \sum_{\substack{l=1 \\ \text{odd} }}^{\tau_N(t)} 
        \alpha_n^l (1+O(N^{-1})) \frac{1}{l!} (t+1)^{l-1} (1+B_n)^l \notag\\
&\geq \sum_{l=0}^{\tau_N(t)} (-\alpha_n)^l (1+O(N^{-1})) 
        \frac{1}{l!} t^l \1{E}
        - \left( \sum_{s=1}^{\tau_N(t)} c_N(s)^2 \right)
        \frac{1}{2} \alpha_n^2 \exp[ \alpha_n (1+O(N^{-1})) (t+1) ]\notag\\
    &\qquad- c_N(\tau_N(t)) \exp[ \alpha_n (1+O(N^{-1})) (t+1) ] \notag\\
    &\qquad- \left( \sum_{s=1}^{\tau_N(t)} D_N(s) \right)
        \exp[ \alpha_n (1+O(N^{-1})) (t+1) (1+B_n) ].
\end{align}
Now, taking the expectation and limit, and applying \citet[Equations (3.3)--(3.5)]{brown2021} and Lemma~?? \seb{(Lemma 2 in the messy weakconv note; not written up here yet)},
\begin{align}
\lim_{N\to\infty} \E \left[ \prod_{r=1}^{\tau_N(t)} (1-p_r) \right]
&\geq \sum_{l=0}^{\infty} (-\alpha_n)^l (1+O(N^{-1})) \frac{1}{l!} t^l 
        \lim_{N\to\infty} \Prob\left[ \{\tau_N(t) \geq l\} \cap E \right] \notag\\
    &\qquad- \lim_{N\to\infty} \E \left[ \sum_{s=1}^{\tau_N(t)} c_N(s)^2 \right]
        \frac{1}{2} \alpha_n^2 \exp[ \alpha_n (t+1) ]\notag\\
    &\qquad- \lim_{N\to\infty} \E \left[ c_N(\tau_N(t)) \right] 
        \exp[ \alpha_n (t+1) ] \notag\\
    &\qquad- \lim_{N\to\infty} \E \left[ \sum_{s=1}^{\tau_N(t)} D_N(s) \right]
        \exp[ \alpha_n (t+1) (1+B_n) ] \notag\\
&= \sum_{l=0}^{\infty} (-\alpha_n)^l \frac{1}{l!} t^l
= e^{-\alpha_n t}. \label{eq:029}
\end{align}
Combining the upper and lower bounds in \eqref{eq:022} and \eqref{eq:029} respectively concludes the proof.
\end{proof}



\bibliography{../smc.bib}
\end{document}