\documentclass[fleqn]{article}
\usepackage[utf8]{inputenc}
\usepackage[margin=2.5cm]{geometry}

% bibliography
\usepackage[round, sort&compress]{natbib}
\usepackage{har2nat}
\bibliographystyle{agsm}

% custom header/footer
\usepackage{fancyhdr}
\pagestyle{fancy}
\renewcommand{\headrulewidth}{0pt}
\fancyhf{}
\rfoot{\textsf{\thepage}}
\lfoot{\textsf{Suzie Brown}}

% maths / theorems
\usepackage{amsmath}
\usepackage{amssymb}
\usepackage{amsthm}
\newtheorem{thm}{Theorem}
\newtheorem{lemma}{Lemma}
\newtheorem{remark}{Remark}
\newtheorem{corollary}{Corollary}
\newtheorem{conj}{Conjecture}
\newtheorem{prop}{Proposition}
\theoremstyle{definition}
\newtheorem{defn}{Definition}

% useful math symbols
\newcommand{\N}{\mathbb{N}}
\newcommand{\Prob}{\mathbb{P}}
\newcommand{\E}{\mathbb{E}}
\newcommand{\V}{\operatorname{Var}}
\newcommand{\eqdist}{\overset{d}{=}}
\newcommand{\I}[1]{\mathbb{I}_{\{#1\}}}
\newcommand{\Ntoinfty}{\overset{N\to\infty}{\longrightarrow}}
\newcommand{\limNtoinfty}{\underset{N\to\infty}{\lim}}
\newcommand\indep{\protect\mathpalette{\protect\independenT}{\perp}}
\def\independenT#1#2{\mathrel{\rlap{$#1#2$}\mkern2mu{#1#2}}}

% distributions
\newcommand{\Cat}{\operatorname{Categorical}}
\newcommand{\Unif}{\operatorname{Uniform}}
\newcommand{\Mn}{\operatorname{Multinomial}}
\newcommand{\Bin}{\operatorname{Binomial}}

% project-specific symbols
\newcommand{\F}{\mathcal{F}_{t-1}}
\newcommand{\vt}[2][t]{\nu_{#1}^{(#2)}}
\newcommand{\wt}[2][t]{w_{#1}^{(#2)}}
\newcommand{\wbar}[2][t]{\bar{w}_{#1}^{(#2)}}
\newcommand{\vttilde}[2][t]{\tilde{\nu}_{#1}^{(#2)}}
\newcommand{\flnw}{\lfloor Nw_i \rfloor }

\title{Conditional SMC --- with updated assumptions}
\author{Suzie Brown}
\date{\today}

\begin{document}
\maketitle
\thispagestyle{fancy}

\begin{thm}\label{thm:mn_newassns}
Under the time scaling of \citet[Theorem 1]{koskela2018} and the conditions of \citet[Lemma 3]{koskela2018}, genealogies of SMC algorithms with multinomial resampling converge to Kingman's $n$-coalescent in the sense of finite-dimensional distributions as $N\to\infty$.
\end{thm}

\begin{proof}
The standing assumption holds by exchangeability of the Multinomial distribution.
We also need to show that there exists a deterministic sequence $(b_N)_{N\in\N}$ such that $\limNtoinfty b_N =0$ and
\begin{equation}\label{eq:mn_ratiobound}
\frac{\frac{1}{(N)_3}\sum_{i=1}^N \E[(\vt{i})_3 |\F]}{\frac{1}{(N)_2} \sum_{i=1}^N \E[(\vt{i})_2 |\F]} \leq b_N
\end{equation}
for all $N \in \N$. 
For the denominator, we apply \citet[Lemma 3]{koskela2018} directly to obtain, for some constants $a\geq \varepsilon\geq0$,
\begin{equation*}
\sum_{i=1}^N \E[(\vt{i})_2 |\F] \geq \frac{(N)_2 \varepsilon^4}{Na^4}
\end{equation*}
For the numerator, we use that $\vt{i} \longrightarrow (\vt{i})_3$ is $\{i\}$-increasing, along with the argument from the proof of \citet[Lemma 3]{koskela2018}, to obtain
\begin{equation*}
\sum_{i=1}^N \E[(\vt{i})_3 |\F] \leq \sum_{i=1}^N  \E[(\tilde{a}_t^{(i)})_3]
\end{equation*}
where
\begin{equation}
\tilde{a}_t^{(j)} \sim^{iid} \Cat \left( \left(\frac{a}{\varepsilon}\right)^{\I{i=1}-\I{i\neq 1}}, \left(\frac{a}{\varepsilon}\right)^{\I{i=2}-\I{i\neq 2}}, \dots, \left(\frac{a}{\varepsilon}\right)^{\I{i=N}-\I{i\neq N}} \right)
\end{equation}
We can calculate the expectation for $\tilde{a}_t^{(1:N)}$, so we have
\begin{align*}
\sum_{i=1}^N \E[(\vt{i})_3 |\F] &\leq 
(N)_3 \left( \frac{1}{(N-1)\varepsilon/a + a/\varepsilon} \right)^3 \left[ (N-1)\left(\frac{\varepsilon}{a}\right)^3 + \left(\frac{a}{\varepsilon}\right)^3 \right] \\
&= \frac{(N)_3}{\left((N-1)\varepsilon^2 + a^2\right)^3}\left(a^6 + (N-1)\varepsilon^6\right) \\
&\leq \frac{(N)_3}{N^3\varepsilon^6} (Na^6) = \frac{(N)_3}{N^2} \frac{a^6}{\varepsilon^6}
\end{align*}
where the last inequality follows because $a\geq \varepsilon$.
Putting these together, we can bound the ratio \eqref{eq:mn_ratiobound} above by
\begin{equation*}
b_N := \frac{(N)_3 \frac{(N)_3}{N^2} \frac{a^6}{\varepsilon^6}}{(N)_2 \frac{(N)_2 \varepsilon^4}{Na^4}} = \frac{1}{N}\frac{a^{10}}{\varepsilon^{10}} \quad \Ntoinfty 0
\end{equation*}
We conclude the result by applying Theorem ? [the KJJS Thm1 with updated assns].
\end{proof}

\begin{thm}\label{thm:CSMC_newassns}
Under the time scaling of \citet[Theorem 1]{koskela2018} and the conditions of \citet[Lemma 3]{koskela2018}, genealogies of conditional SMC algorithms with multinomial resampling converge to Kingman's $n$-coalescent in the sense of finite-dimensional distributions as $N\to\infty$.
\end{thm}

\begin{proof}
Denote the vector of particle weights $\wt{1:N} = (\wt{1}, \wt{2}, \dots, \wt{N})$, and let $\vttilde{1:N} = (\vttilde{1}, \vttilde{2}, \dots, \vttilde{N})$ denote the associated offspring counts under conditional SMC. Assuming WLOG that the immortal particle has index 1, the offspring counts are distributed according to
\begin{equation*}
\vttilde{1:N} \mid \wt{1:N} \eqdist (1,0,0,\dots, 0) + \Mn(N-1, \wt{1:N})
\end{equation*}
The standing assumption holds by exchangeability of the offspring assignments in Algorithm \ref{alg:condSMC}. 
Like for Theorem \ref{thm:mn_newassns}, we need to show that
\begin{equation}\label{eq:csmc_ratiobound}
\frac{\frac{1}{(N)_3}{\sum_{i=1}^N \E[(\vttilde{i})_3 |\F}}{\frac{1}{(N)_2} \sum_{i=1}^N \E[(\vttilde{i})_2 |\F]} \leq b_N
\end{equation}
for some deterministic sequence $b_N \Ntoinfty 0$. For the denominator, we have
\begin{align*}
\sum_{i=1}^N \E[(\vttilde{i})_2 |\F]
&=  \E\left[ (\vttilde{1})_2 |\F \right] + \sum_{i=2}^{N} \E\left[ (\vttilde{i})_2 |\F \right] \\
&= (N-1)_2\E[(\wt{1})^2 |\F] + 2(N-1)\E[\wt{1} |\F] + \sum_{i=2}^{N} (N-1)_2\E[(\wt{i})^2 |\F] \\
&= (N-1)_2 \sum_{i=1}^{N} \E[(\wt{i})^2 |\F] + 2(N-1) \E[\wt{1} |\F] 
\end{align*}
using that $(X+1)_2 = (X)_2 + 2(X)_1$ and the factorial moments of the Multinomial distribution \citep{mosimann1962}.
For the numerator, we have
\begin{align*}
\sum_{i=1}^N \E[(\vttilde{i})_3 |\F]
&=  \E\left[ (\vttilde{1})_3 |\F \right] + \sum_{i=2}^{N} \E\left[ (\vttilde{i})_3 |\F \right] \\
&= (N-1)_3\E[(\wt{1})^3 |\F] + 3(N-1)_2\E[(\wt{1})^2 |\F] + \sum_{i=2}^{N} (N-1)_3\E[(\wt{i})^3 |\F] \\
&= (N-1)_3 \sum_{i=1}^{N} \E[(\wt{i})^3 |\F] + 3(N-1)_2 \E[(\wt{1})^2 |\F] 
\end{align*}
using similarly that $(X+1)_3 = (X)_3 + 3(X)_2$.
Combining these expressions, the ratio in \eqref{eq:csmc_ratiobound} becomes
\begin{align*}
\frac{\frac{1}{(N)_3}\sum_{i=1}^N \E[(\vttilde{i})_3 |\F]}{\frac{1}{(N)_2} \sum_{i=1}^N \E[(\vttilde{i})_2 |\F]}
&= \frac{1}{N-2} \frac{(N-1)_3 \sum_{i=1}^{N} \E[(\wt{i})^3 |\F] + 3(N-1)_2 \E[(\wt{1})^2 |\F] }{(N-1)_2 \sum_{i=1}^{N} \E[(\wt{i})^2 |\F] + 2(N-1) \E[\wt{1} |\F]} \\
&\leq \frac{1}{N-2} \frac{(N-1)_3 \sum_{i=1}^{N} \E[(\wt{i})^3 |\F]}{(N-1)_2 \sum_{i=1}^{N} \E[(\wt{i})^2 |\F]} + \frac{1}{N-2} \frac{3(N-1)_2 \E[(\wt{1})^2 |\F]}{(N-1)_2 \sum_{i=1}^{N} \E[(\wt{i})^2 |\F]} \\
&\leq \frac{1}{N-2} \frac{(N-1)_3 \sum_{i=1}^{N} \E[(\wt{i})^3 |\F]}{(N-1)_2 \sum_{i=1}^{N} \E[(\wt{i})^2 |\F]} + \frac{1}{N-2} \frac{3(N-1)_2 \E[(\wt{1})^2 |\F]}{(N-1)_2 \E[(\wt{1})^2 |\F]} \\
&<  \frac{1}{N-2} \frac{\sum_{i=1}^{N} \E[(\vt{i})_3 |\F]}{\sum_{i=1}^{N} \E[(\vt{i})_2 |\F]} + \frac{3}{N-2}
\end{align*}
where the last inequality holds because $\frac{(N-1)_3}{(N-1)_2} = N-3 < N-2 = \frac{(N)_3}{(N)_2}$.
Then, using Theorem \ref{thm:mn_newassns}, we can bound this by
\begin{equation*}
b_N := \frac{1}{N}\frac{a^6}{\varepsilon^6} + \frac{3}{N-2} \quad \Ntoinfty 0
\end{equation*}
as required, where $a$ and $\varepsilon$ are constants defined in the conditions of \citet[Lemma 3]{koskela2018}.
We conclude the result by applying Theorem ? [the KJJS Thm1 with updated assns].
\end{proof}

\bibliography{../smc.bib}
\end{document}